extraction/theories/TypeAnnotations.v
@@ -1,0 +1,510 @@
+From ConCert.Extraction Require Import Annotations.
+From ConCert.Extraction Require Import Aux.
+From ConCert.Extraction Require Import Erasure.
+From ConCert.Extraction Require Import ExAst.
+From ConCert.Extraction Require Import Extraction.
+From ConCert.Extraction Require Import Optimize.
+From ConCert.Extraction Require Import ResultMonad.
+From Coq Require Import List.
+From Coq Require Import VectorDef.
+From Equations Require Import Equations.
+From MetaCoq.Erasure Require Import EArities.
+From MetaCoq.Erasure Require Import Extract.
+From MetaCoq.Erasure Require SafeErasureFunction.
+From MetaCoq.PCUIC Require Import PCUICAst.
+From MetaCoq.PCUIC Require Import PCUICInversion.
+From MetaCoq.PCUIC Require Import PCUICLiftSubst.
+From MetaCoq.PCUIC Require Import PCUICGeneration.
+From MetaCoq.PCUIC Require Import PCUICTyping.
+From MetaCoq.PCUIC Require Import PCUICValidity.
+From MetaCoq.PCUIC Require Import PCUICSafeLemmata.
+From MetaCoq.SafeChecker Require Import PCUICSafeRetyping.
+From MetaCoq.Template Require Import Kernames.
+
+Import VectorNotations.
+Import ListNotations.
+
+Open Scope list.
+
+Section fix_env.
+Opaque flag_of_type erase_type.
+
+Context (Σ : global_env_ext).
+Context (wfextΣ : ∥wf_ext Σ∥).
+Lemma wfΣ : ∥wf Σ∥.
+Proof. now sq. Qed.
+
+Section annotate.
+  Context {A : Type}.
+  Context (annotate_types :
+             forall Γ t (Ht : welltyped Σ Γ t) et (er : erases Σ Γ t et), annots A et).
+
+  Equations? (noeqns) annotate_branches
+           Γ
+           (brs : list (nat × term))
+           (ebrs : list (nat × E.term))
+           (wf : Forall2 (fun '(_, t) '(_, et) => welltyped Σ Γ t /\ erases Σ Γ t et) brs ebrs)
+    : bigprod (annots A ∘ snd) ebrs by struct ebrs :=
+    annotate_branches Γ _ [] _ := tt;
+    annotate_branches Γ ((_, t) :: brs) ((_, et) :: ebrs) wf :=
+      (annotate_types Γ t _ et _, annotate_branches Γ brs ebrs _);
+    annotate_branches _ _ _ _ := !.
+  Proof. all: now depelim wf. Qed.
+
+  Equations? (noeqns) annotate_defs
+           Γ
+           (defs : list (def term))
+           (edefs : list (E.def E.term))
+           (wf : Forall2 (fun d ed => welltyped Σ Γ (dbody d) /\ erases Σ Γ (dbody d) (E.dbody ed))
+                         defs edefs)
+    : bigprod (annots A ∘ E.dbody) edefs by struct edefs :=
+    annotate_defs Γ _ [] _ := tt;
+    annotate_defs Γ (d :: defs) (ed :: edefs) wf :=
+      (annotate_types Γ (dbody d) _ (E.dbody ed) _, annotate_defs Γ defs edefs _);
+    annotate_defs _ _ _ _ := !.
+  Proof. all: now depelim wf. Qed.
+End annotate.
+
+Fixpoint vec_repeat {A} (a : A) (n : nat) : Vector.t A n :=
+  match n with
+  | 0 => []%vector
+  | S n => (a :: vec_repeat a n)%vector
+  end.
+
+Program Definition erase_type_of Γ t (wt : welltyped Σ Γ t) : box_type :=
+  let ty := type_of Σ wfΣ _ Γ t wt in
+  let flag := flag_of_type Σ wfextΣ Γ ty _ in
+  if is_arity flag then
+    TBox
+  else
+    (erase_type_aux Σ wfextΣ Γ (vec_repeat RelOther #|Γ|) ty _ None).2.
+Next Obligation.
+  destruct wfextΣ as [[]].
+  now constructor.
+Qed.
+Next Obligation.
+  unfold type_of.
+  destruct infer as (ty & [(typ & ?)]).
+  cbn.
+  destruct wfΣ.
+  constructor.
+  eapply validity_term; eauto.
+Qed.
+Next Obligation.
+  unfold type_of in *.
+  destruct infer as (ty & [(typ & ?)]).
+  cbn in *.
+  destruct wfΣ.
+  eapply validity_term in typ; eauto.
+  destruct typ.
+  - now apply nIs_conv_to_Arity_isWfArity_elim in H.
+  - now constructor.
+Qed.
+
+Equations? (noeqns) annotate_types
+         (Γ : context)
+         (t : term) (wt : welltyped Σ Γ t)
+         (et : E.term)
+         (er : erases Σ Γ t et) : annots box_type et by struct et :=
+(* For some reason 'with' hangs forever so we need 'where' here *)
+annotate_types Γ t wt et er := annot (erase_type_of Γ t wt) et t wt er
+where annot
+        (bt : box_type)
+        (et : E.term)
+        (t : term) (wt : welltyped Σ Γ t)
+        (er : erases Σ Γ t et) : annots box_type et := {
+annot bt E.tBox _ _ _ => bt;
+annot bt (E.tRel _) _ _ _ => bt;
+annot bt (E.tVar _) _ _ _ => bt;
+annot bt (E.tEvar _ ets) t wt er => !;
+annot bt (E.tLambda na eB) (tLambda na' A B) wt er => (bt, annotate_types (Γ,, vass na' A) B _ eB _);
+annot bt (E.tLetIn na eb eb') (tLetIn na' b ty b') wt er =>
+  (bt, (annotate_types Γ b _ eb _, annotate_types (Γ,, vdef na' b ty) b' _ eb' _));
+annot bt (E.tApp ehd earg) (tApp hd arg) wt er =>
+  (bt, (annotate_types Γ hd _ ehd _, annotate_types Γ arg _ earg _));
+annot bt (E.tConst _) _ wt er => bt;
+annot bt (E.tConstruct _ _) _ wt er => bt;
+annot bt (E.tCase _ ediscr ebrs) (tCase _ _ discr brs) wt er =>
+  (bt, (annotate_types Γ discr _ ediscr _, annotate_branches annotate_types Γ brs ebrs _));
+annot bt (E.tProj _ et) (tProj _ t) wt er => (bt, annotate_types Γ t _ et _);
+annot bt (E.tFix edefs _) (tFix defs _) wt er =>
+  (bt, annotate_defs annotate_types (Γ,,, fix_context defs) defs edefs _);
+annot bt (E.tCoFix edefs _) (tCoFix defs _) wt er =>
+  (bt, annotate_defs annotate_types (Γ,,, fix_context defs) defs edefs _);
+annot bt _ _ wt er => !
+}.
+Proof.
+  all: try solve [inversion er; auto].
+  all: destruct wt.
+  all: destruct wfextΣ as [[]].
+  - depelim er.
+    now apply inversion_Evar in X.
+  - apply inversion_Lambda in X as (? & ? & ? & ? & ?); auto.
+    econstructor; eauto.
+  - apply inversion_LetIn in X as (?&?&?&?&?&?); auto.
+    econstructor; eauto.
+  - apply inversion_LetIn in X as (?&?&?&?&?&?); auto.
+    econstructor; eauto.
+  - apply inversion_App in X as (?&?&?&?&?&?); auto.
+    econstructor; eauto.
+  - apply inversion_App in X as (?&?&?&?&?&?); auto.
+    econstructor; eauto.
+  - apply inversion_Case in X as (?&?&?&?&?&?&?&?&?&?&?&?&?&?&?&?&?); auto.
+    econstructor; eauto.
+  - apply inversion_Case in X as (?&?&?&?&?&?&?&?&?&?&?&?&?&?&?&?&?); auto.
+    depelim er.
+    clear -a X.
+    induction X in x5, a, X |- *; [constructor|].
+    depelim a.
+    constructor; eauto.
+    destruct x, y0.
+    destruct r.
+    destruct p as ((?&?)&?).
+    cbn in *.
+    split; [|now auto].
+    econstructor; eauto.
+  - apply inversion_Proj in X as (?&?&?&?&?&?&?&?&?); auto.
+    econstructor; eauto.
+  - apply inversion_Fix in X as (?&?&?&?&?&?&?); auto.
+    depelim er.
+    clear -a0 X.
+    eapply All2_All_mix_left in X; eauto.
+    clear -X.
+    revert X.
+    generalize (Γ,,, fix_context defs).
+    clear Γ.
+    intros Γ a.
+    induction a; [now constructor|].
+    constructor; [|now eauto].
+    destruct r as ((? & ?) & ? & ? & ?).
+    split; [|now auto].
+    econstructor; eauto.
+  - apply inversion_CoFix in X as (?&?&?&?&?&?&?); auto.
+    depelim er.
+    clear -a0 X.
+    eapply All2_All_mix_left in X; eauto.
+    clear -X.
+    revert X.
+    generalize (Γ,,, fix_context defs).
+    clear Γ.
+    intros Γ a.
+    induction a; [now constructor|].
+    constructor; [|now eauto].
+    destruct r as (? & ? & ? & ?).
+    split; [|now auto].
+    econstructor; eauto.
+Qed.
+
+Definition annotate_types_erase_constant_decl cst wt :
+  match erase_constant_decl Σ wfextΣ cst wt with
+  | Ok (inl cst) => constant_body_annots box_type cst
+  | _ => unit
+  end.
+Proof.
+  unfold erase_constant_decl.
+  destruct flag_of_type.
+  cbn in *.
+  destruct is_arity.
+  - destruct is_sort; [|exact tt].
+    destruct cst; cbn.
+    destruct cst_body; exact tt.
+  - destruct cst; cbn.
+    destruct cst_body; [|exact tt].
+    cbn.
+    apply (annotate_types [] t); [|apply SafeErasureFunction.erases_erase].
+    cbn in *.
+    destruct wt.
+    econstructor; eauto.
+Defined.
+
+Definition annotate_types_erase_global_decl kn decl wt :
+  match erase_global_decl Σ wfextΣ kn decl wt with
+  | Ok decl => global_decl_annots box_type decl
+  | _ => unit
+  end.
+Proof.
+  unfold erase_global_decl.
+  destruct decl; [|exact tt].
+  cbn.
+  pose proof (annotate_types_erase_constant_decl c wt).
+  destruct erase_constant_decl; [|exact tt].
+  cbn.
+  destruct t; [|exact tt].
+  exact X.
+Defined.
+
+End fix_env.
+
+Definition annotate_types_erase_global_decls_deps_recursive Σ wfΣ include ignore_deps :
+  match erase_global_decls_deps_recursive Σ wfΣ include ignore_deps with
+  | Ok Σ => env_annots box_type Σ
+  | _ => unit
+  end.
+Proof.
+  revert include.
+  induction Σ; intros include; [exact tt|].
+  cbn in *.
+  destruct a.
+  destruct KernameSet.mem.
+  - cbn.
+    match goal with
+    | |- context[erase_global_decl ?a ?b ?c ?d ?e] =>
+      pose proof (annotate_types_erase_global_decl a b c d e);
+        destruct erase_global_decl
+    end; [|exact tt].
+    match goal with
+    | |- context[erase_global_decls_deps_recursive _ ?prf ?incl _] =>
+      specialize (IHΣ prf incl);
+        destruct erase_global_decls_deps_recursive
+    end; [|exact tt].
+    cbn.
+    exact (X, IHΣ).
+  - match goal with
+    | |- context[erase_global_decls_deps_recursive _ ?prf ?incl _] =>
+      specialize (IHΣ prf incl);
+        destruct erase_global_decls_deps_recursive
+    end; [|exact tt].
+    exact IHΣ.
+Defined.
+
+Import EAst.
+Definition annot_dearg_lambdas {A} mask {t} (ta : annots A t)
+  : annots A (dearg_lambdas mask t).
+Proof.
+  revert t ta mask.
+  fix f 1.
+  intros [] ta mask; cbn in *; try exact ta.
+  - destruct mask; [exact ta|].
+    destruct b.
+    + apply annot_subst1; [exact ta.1|].
+      apply (f _ ta.2).
+    + exact (ta.1, f _ ta.2 _).
+  - exact (ta.1, (ta.2.1, f _ ta.2.2 _)).
+Defined.
+
+Definition annot_dearg_single
+           mask
+           {hd}
+           (hda : annots box_type hd)
+           {args}
+           (argsa : All (fun t => box_type * annots box_type t) args)
+  : annots box_type (dearg_single mask hd args).
+Proof.
+  revert hd hda args argsa.
+  induction mask; intros hd hda args argsa; cbn.
+  - apply annot_mkApps; assumption.
+  - destruct a.
+    + (* arg is being removed but overall type does not change. *)
+      destruct argsa.
+      * (* there is no arg. Lambda has original type so body has type of codomain *)
+        refine (annot hda, _).
+        apply IHmask; [|exact All_nil].
+        apply annot_lift.
+        (* type of body is now the codomain *)
+        exact (map_annot
+                 (fun bt =>
+                    match bt with
+                    | TArr _ cod => cod
+                    | _ => bt
+                    end) hda).
+      * (* arg was removed, new type is codomain *)
+        apply IHmask; [|exact argsa].
+        exact (map_annot
+                 (fun bt =>
+                    match bt with
+                    | TArr _ cod => cod
+                    | _ => bt
+                    end) hda).
+    + destruct argsa.
+      * refine (annot hda, _).
+        apply IHmask; [|exact All_nil].
+        cbn.
+        exact (match annot hda with
+                | TArr dom cod => (cod, (annot_lift _ _ hda, dom))
+                | t => (t, (annot_lift _ _ hda, t))
+                end).
+      * apply IHmask; [|exact argsa].
+        exact (match annot hda with
+               | TArr dom cod => (cod, (hda, p.2))
+               | t => (t, (hda, p.2))
+               end).
+Defined.
+
+Definition annot_dearg_case_branches
+           {A}
+           mm i
+           {brs} (brsa : bigprod (annots A ∘ snd) brs)
+  : bigprod (annots A ∘ snd) (dearg_case_branches mm i brs).
+Proof.
+  destruct mm; [|exact brsa].
+  cbn.
+  apply bigprod_mapi_rec; [|exact brsa].
+  intros.
+  apply annot_dearg_lambdas.
+  exact X.
+Defined.
+
+Definition annot_dearg_aux
+           im cm
+           {args : list term}
+           (argsa : All (fun t => box_type * annots box_type t) args)
+           {t : term}
+           (ta : annots box_type t) : annots box_type (dearg_aux im cm args t).
+Proof.
+  revert args argsa t ta.
+  fix f 3.
+  intros args argsa [] ta; cbn.
+  - exact (annot_mkApps ta argsa).
+  - exact (annot_mkApps ta argsa).
+  - exact (annot_mkApps ta argsa).
+  - apply annot_mkApps; [|exact argsa].
+    cbn in *.
+    refine (ta.1, bigprod_map _ ta.2).
+    apply f.
+    exact All_nil.
+  - apply annot_mkApps; [|exact argsa].
+    exact (ta.1, f _ All_nil _ ta.2).
+  - apply annot_mkApps; [|exact argsa].
+    exact (ta.1, (f _ All_nil _ ta.2.1, f _ All_nil _ ta.2.2)).
+  - apply f; [|exact ta.2.1].
+    apply All_cons; [|exact argsa].
+    exact (ta.1, f _ All_nil _ ta.2.2).
+  - exact (annot_dearg_single _ ta argsa).
+  - exact (annot_dearg_single _ ta argsa).
+  - destruct p.
+    refine (annot_mkApps _ argsa).
+    cbn in *.
+    refine (ta.1, _).
+    refine (f _ All_nil _ ta.2.1, _).
+    apply annot_dearg_case_branches.
+    apply bigprod_map; [|exact ta.2.2].
+    intros.
+    exact (f _ All_nil _ X).
+  - destruct p as ((? & ?) & ?).
+    refine (annot_mkApps _ argsa).
+    refine (ta.1, _).
+    exact (f _ All_nil _ ta.2).
+  - refine (annot_mkApps _ argsa).
+    refine (ta.1, _).
+    fold (annots box_type).
+    apply bigprod_map; [|exact ta.2].
+    intros.
+    exact (f _ All_nil _ X).
+  - refine (annot_mkApps _ argsa).
+    refine (ta.1, _).
+    fold (annots box_type).
+    apply bigprod_map; [|exact ta.2].
+    intros.
+    exact (f _ All_nil _ X).
+Defined.
+
+Definition annot_dearg im cm {t : term} (ta : annots box_type t) : annots box_type (dearg im cm t) :=
+  annot_dearg_aux im cm All_nil ta.
+
+Definition annot_debox_type_decl Σ {decl} (a : global_decl_annots box_type decl)
+  : global_decl_annots box_type (debox_type_decl Σ decl).
+Proof.
+  unfold debox_type_decl.
+  destruct decl; [|exact a|exact a].
+  cbn in *.
+  (* we have removed type variables from inductives, so adjust type annotations similarly *)
+  unfold constant_body_annots in *.
+  cbn.
+  destruct Ex.cst_body; [|exact tt].
+  exact (map_annots (debox_box_type Σ) a).
+Defined.
+
+Definition annot_debox_env_types {Σ} (a : env_annots box_type Σ)
+  : env_annots box_type (debox_env_types Σ).
+Proof.
+  unfold debox_env_types.
+  apply bigprod_map; [|exact a].
+  intros.
+  apply annot_debox_type_decl.
+  exact X.
+Defined.
+
+Definition annot_dearg_cst im cm kn {cst} (a : constant_body_annots box_type cst)
+  : constant_body_annots box_type (dearg_cst im cm kn cst).
+Proof.
+  red in a |- *.
+  unfold dearg_cst.
+  cbn in *.
+  destruct Annotations.Ex.cst_body; [|exact tt].
+  cbn.
+  apply annot_dearg.
+  apply annot_dearg_lambdas.
+  exact a.
+Defined.
+
+Definition annot_dearg_decl im cm kn {decl} (a : global_decl_annots box_type decl) :
+  global_decl_annots box_type (dearg_decl im cm kn decl).
+Proof.
+  unfold dearg_decl.
+  destruct decl; try exact a.
+  cbn.
+  apply annot_dearg_cst.
+  exact a.
+Defined.
+
+Definition annot_dearg_env im cm {Σ} (a : env_annots box_type Σ)
+  : env_annots box_type (dearg_env im cm Σ).
+Proof.
+  apply bigprod_map; [|exact a].
+  intros ((? & ?) & ?) ?.
+  cbn in *.
+  apply annot_dearg_decl.
+  exact X.
+Defined.
+
+Definition annot_extract_pcuic_env params Σ wfΣ include ignore :
+  match extract_pcuic_env params Σ wfΣ include ignore with
+  | Ok Σ => env_annots box_type Σ
+  | _ => unit
+  end.
+Proof.
+  unfold extract_pcuic_env.
+  pose proof (annotate_types_erase_global_decls_deps_recursive Σ wfΣ include ignore).
+  destruct erase_global_decls_deps_recursive; cbn; [|exact tt].
+  destruct dearg_args; [|exact X].
+  destruct (_ && _); [exact tt|].
+  destruct analyze_env.
+  destruct (_ && _); [exact tt|].
+  destruct (_ && _); [exact tt|].
+  apply annot_debox_env_types.
+  apply annot_dearg_env.
+  exact X.
+Defined.
+
+Definition annot_extract_pcuic_env_sig
+           (params : extract_pcuic_params)
+           (Σ : P.global_env) (wfΣ : ∥wf Σ∥)
+           (include : KernameSet.t)
+           (ignore : kername -> bool) : option (∑ Σ, env_annots box_type Σ).
+Proof.
+  pose proof (annot_extract_pcuic_env params Σ wfΣ include ignore).
+  destruct extract_pcuic_env; [|exact None].
+  exact (Some (t; X)).
+Defined.
+
+Definition annot_extract_template_env params Σ include ignore :
+  match extract_template_env params Σ include ignore with
+  | Ok Σ => env_annots box_type Σ
+  | _ => unit
+  end.
+Proof.
+  unfold extract_template_env.
+  destruct check_wf_env_func; [|exact tt].
+  apply annot_extract_pcuic_env.
+Defined.
+
+Definition annot_extract_template_env_sig
+           (params : extract_template_env_params)
+           (Σ : Ast.global_env)
+           (include : KernameSet.t)
+           (ignore : kername -> bool) : option (∑ Σ, env_annots box_type Σ).
+Proof.
+  pose proof (annot_extract_template_env params Σ include ignore).
+  destruct extract_template_env; [|exact None].
+  exact (Some (t; X)).
+Defined.
